boringssl_fips_20180730/digest_protocol_verif.v
@@ -1,0 +1,1522 @@
+Require Import VST.floyd.proofauto.
+Require Import boringssl_fips_20180730.spec_mem.
+Require Import boringssl_fips_20180730.digest.
+
+Require Export boringssl_fips_20180730.digest_model.
+Require Import boringssl_fips_20180730.spec_digest_base.
+Require Import boringssl_fips_20180730.spec_digest.
+Require Import boringssl_fips_20180730.digest_protocol_spec.
+Require Import boringssl_fips_20180730.verif_digest.
+Definition ConcGprog: funspecs := EVP_DigestInit_ex_SPEC :: EVP_DigestUpdate_SPEC :: Gprog_EVPMDCTX_1. (*and many more -- all specs from spec_digest*)
+
+Module EVP_MD_CTX_Protocol <: EVP_MD_CTX_Protocol_TP.
+Variant State :=
+  Allocated: State
+| Raw: State
+| Empty: forall (D:EVP_MD) (d:val), State
+| Hashed: forall (DC: MD_with_content) (d:val), State
+| Full: forall (D: EVP_MD) (d:val), State.
+
+Definition MDCTXAllocated p : mpred := 
+  OPENSSL_malloc_token 16 p * data_at_ Ews (Tstruct _env_md_ctx_st noattr) p.
+
+Definition MDCTXRaw p : mpred := 
+  OPENSSL_malloc_token 16 p * CTX_NULL Ews p.
+
+(*
+Definition MD_proper D := sizeof (struct_of_MD D) = EVP_MD_rec_ctx_size D /\ 
+                    0 < sizeof (struct_of_MD D) <= Int.max_unsigned.
+*)
+Definition MDCTXEmpty (D:EVP_MD) (d p:val): mpred :=
+  EX md:val, (*!!(MD_proper D) &&*) 
+        EVP_MD_CTX_NNnode Ews (d,(md,(nullval,nullval))) p *
+        OPENSSL_malloc_token 16 p *
+        MD_state Ews (INI D) md * 
+        OPENSSL_malloc_token (ctx_size_of_MD D) md.
+
+Definition MDCTXHashed (DC: MD_with_content) (d p:val): mpred :=
+  EX md:val, (*!!(MD_proper D)  &&*) 
+        EVP_MD_CTX_NNnode Ews (d,(md,(nullval,nullval))) p *
+        OPENSSL_malloc_token 16 p *
+        MD_state Ews DC md * 
+        OPENSSL_malloc_token (ctx_size_of_MD (__EVP_MD DC)) md.
+
+Definition MDCTXFull D d p: mpred := EX md:val,
+  EVP_MD_CTX_NNnode Ews (d,(md,(nullval,nullval))) p *
+  OPENSSL_malloc_token 16 p *
+  postFin Ews D md *
+  OPENSSL_malloc_token (ctx_size_of_MD D) md.
+
+Definition MDCTX (s: State): val -> mpred :=
+  match s with 
+  Allocated => MDCTXAllocated
+| Raw => MDCTXRaw
+| Empty D d => MDCTXEmpty D d
+| Hashed DC d => MDCTXHashed DC d
+| Full D d => MDCTXFull D d
+  end.
+
+Lemma RawAllocated: forall p, MDCTX Raw p |-- MDCTX Allocated p.
+Proof. intros; simpl. unfold MDCTXRaw, MDCTXAllocated, CTX_NULL. cancel. Qed.
+
+Lemma HashedFull: forall DC d p, MDCTX (Hashed DC d) p |-- MDCTX (Full (__EVP_MD DC) d) p.
+Proof. intros; simpl. unfold MDCTXHashed, MDCTXFull, EVP_MD_CTX_NNnode.
+  Intros md; Exists md. (* sep_apply (MD_StateFIN DC md). entailer!. *)
+  destruct DC. simpl. unfold postFin, MD_state. Intros c. Exists c. entailer!. Qed.
+
+Lemma Empty_HashedIni: forall D d p, MDCTX (Empty D d) p |-- MDCTX (Hashed (INI D) d) p.
+Proof. intros; simpl. unfold MDCTXHashed, MDCTXEmpty. simpl; trivial. Qed.
+
+Lemma EmptyFull: forall D d p, MDCTX (Empty D d) p |-- MDCTX (Full D d) p.
+Proof. intros. sep_apply (Empty_HashedIni D d p). apply HashedFull. Qed.
+
+Definition LEAK (c:State) :mpred :=
+  match c with
+  Allocated => emp
+| Raw => emp
+| Empty D d => EX md:_, MD_state Ews (INI D) md * OPENSSL_malloc_token (ctx_size_of_MD D) md
+| Hashed DC d => EX md:_, MD_state Ews DC md * OPENSSL_malloc_token (ctx_size_of_MD (__EVP_MD DC)) md
+| Full D d => EX md:_, EX data:type_with_content, (*MD_state Ews (Build_MD_with_content D data) md*)
+                                  (*data_block Ews data md *)
+                                  data_at Ews (__type data) (__values data) md * 
+                                  OPENSSL_malloc_token (ctx_size_of_MD D) md
+  end.
+
+Lemma AnyAllocated c p: MDCTX c p |-- MDCTX Allocated p * LEAK c.
+Proof. unfold LEAK. destruct c; try cancel. apply  RawAllocated.
++ simpl. unfold MDCTXEmpty, MDCTXAllocated, EVP_MD_CTX_NNnode. Intros md. Exists md. cancel.
++ simpl. unfold MDCTXHashed, MDCTXAllocated, EVP_MD_CTX_NNnode. Intros md. Exists md. cancel.
++ simpl. unfold MDCTXFull, MDCTXAllocated, EVP_MD_CTX_NNnode. Intros md. Exists md. cancel.
+  unfold postFin. Intros tc. Exists tc. trivial.
+Qed.
+
+Lemma Allocated_valid_ptr: forall p, MDCTX Allocated p |-- valid_pointer p.
+Proof. intros; simpl. unfold MDCTXAllocated. apply sepcon_valid_pointer2.
+  sep_apply (data_at__memory_block Ews (Tstruct _env_md_ctx_st noattr) p); Intros; simpl.
+  sep_apply (memory_block_valid_ptr Ews 16 p); intuition. Qed.
+
+Lemma Allocated_isptr: forall p, MDCTX Allocated p |-- !! isptr p.
+Proof. intros; simpl. unfold MDCTXAllocated. entailer!. Qed.
+
+Lemma Full_valid_ptr: forall D d p, MDCTX (Full D d) p |-- valid_pointer p.
+Proof. intros; simpl. unfold MDCTXFull, EVP_MD_CTX_NNnode; Intros md.
+  apply sepcon_valid_pointer1. do 2 apply sepcon_valid_pointer1. 
+  sep_apply (data_at__memory_block Ews (Tstruct _env_md_ctx_st noattr) p); Intros; simpl.
+  sep_apply (memory_block_valid_ptr Ews 16 p); intuition. Qed.
+
+Lemma Full_isptr: forall D d p, MDCTX (Full D d) p |-- !! isptr p.
+Proof. intros; simpl. unfold MDCTXFull, EVP_MD_CTX_NNnode; Intros md. entailer!. Qed.
+
+Definition EVP_of (c: State): mpred :=
+  match c with
+  Allocated => FF
+| Raw => emp
+| Empty D d => EVP_MD_rep D d
+| Hashed DC d => EVP_MD_rep (__EVP_MD DC) d
+| Full D d => EVP_MD_rep D d
+  end.
+
+Definition EVP_MD_CTX_init_ASPEC := DECLARE _EVP_MD_CTX_init
+   WITH ctx:val
+   PRE [ _ctx OF tptr (Tstruct _env_md_ctx_st noattr) ]
+       PROP () LOCAL (temp _ctx ctx) SEP (MDCTX Allocated ctx)
+   POST [ tvoid ]
+       PROP () LOCAL () SEP (MDCTX Raw ctx).
+
+Lemma subsume_EVP_MD_CTX_init:
+      subsume_funspec (snd EVP_MD_CTX_init_SPEC) (snd EVP_MD_CTX_init_ASPEC).
+Proof.
+apply NDsubsume_subsume.
+{ split; reflexivity. }
+split3; auto.
+intros ctx. Exists (ctx, Ews) (OPENSSL_malloc_token 16 ctx).
+apply andp_right; auto.
++ old_go_lower; entailer.
++ apply prop_right. simplify_Delta; old_go_lower. entailer.
+Qed.
+
+Definition EVP_MD_CTX_copy_ASPEC := DECLARE _EVP_MD_CTX_copy
+  WITH gv:globals, octx:val, ictx:val, c:State
+  PRE [ _out OF (tptr (Tstruct _env_md_ctx_st noattr)),
+        _in OF (tptr (Tstruct _env_md_ctx_st noattr)) ]
+      PROP (c <> Allocated; c <> Raw)
+      LOCAL (gvars gv; temp _out octx; temp _in ictx)
+      SEP (MDCTX c ictx; EVP_of c; MDCTX Allocated octx; mm_inv gv; ERRGV gv)
+  POST [ tint] EX rv:_,
+       PROP ()
+       LOCAL (temp ret_temp rv)
+       SEP (if Val.eq rv nullval then MDCTX Raw octx 
+            else (!!(rv=Vint Int.one) && MDCTX c octx);
+            ERRGV gv; mm_inv gv; MDCTX c ictx; EVP_of c).
+
+Lemma subsume_EVP_MD_CTX_copy:
+      subsume_funspec (snd EVP_MD_CTX_copy_SPEC) (snd EVP_MD_CTX_copy_ASPEC).
+Proof.
+apply NDsubsume_subsume.
+{ split; reflexivity. }
+split3; auto.
+intros [[[gv octx] ictx] c]. specialize WA_WORD_nonneg; intros WAW.
+destruct c; Intros.
++ (*Allocated*) congruence.
++ (*Raw*) congruence.
++ (*Empty*) clear H H0.
+  replace_SEP 0 (MDCTXEmpty D d ictx) by entailer!.
+  unfold MDCTXEmpty; Intros md.
+  replace_SEP 5 (MDCTXAllocated octx) by entailer!.
+  unfold MDCTXAllocated; Intros.
+  unfold EVP_of, EVP_MD_rep; Intros dsh dvals. rename H into Rsh; rename H0 into SZ.
+  rewrite data_at_isptr with (p:=d); Intros.
+  rewrite match_EVP_MD_getctxsize'; Intros; rename H into CTSZ.
+  unfold MD_state, data_block; Intros c. rename H into C. rename H0 into SZmod. rename H1 into HR.
+  Exists (gv, octx, ictx, Ews, cp_default Ews d md nullval dsh dvals Ews c (Int.repr (ctx_size_of_MD D)))
+         (OPENSSL_malloc_token 16 ictx * OPENSSL_malloc_token (ctx_size_of_MD D) md *
+           match_EVP_MD D dvals * OPENSSL_malloc_token 16 octx).
+  apply andp_right; auto.
+  - old_go_lower. entailer!.
+  - apply prop_right. simplify_Delta. Intros rv; Exists rv. old_go_lower.
+    Exists dsh dvals.
+    Intros; subst. entailer!. rewrite sepcon_comm, distrib_orp_sepcon.
+    apply orp_left. 
+    * Intros. subst. rewrite if_true by trivial.
+      unfold MDCTXEmpty, MDCTXRaw, CTX_NULL, MD_state, EVP_MD_CTX_NNnode; cancel.
+      Exists md c. rewrite C; simpl; entailer!.
+    * Intros buf; subst. rewrite if_false by discriminate.
+      unfold MDCTXEmpty, MDCTXRaw, CTX_NULL, EVP_MD_CTX_NNnode, match_EVP_MD.
+      Exists buf md. entailer!. unfold MD_state.
+      Exists c c. rewrite C; simpl; entailer!.
++ (*Hashed*) clear H H0.
+  replace_SEP 0 (MDCTXHashed DC d ictx) by entailer!.
+  unfold MDCTXHashed; Intros md.
+  replace_SEP 5 (MDCTXAllocated octx) by entailer!.
+  unfold MDCTXAllocated, CTX_NULL; Intros.
+  unfold EVP_of, EVP_MD_rep; Intros dsh dvals. rename H into Rsh; rename H0 into SZ.
+  rewrite data_at_isptr with (p:=d); Intros.
+  rewrite match_EVP_MD_getctxsize'; Intros; rename H into CTSZ.
+  unfold MD_state; Intros c; rename H into C. rename H0 into REP.
+  Exists (gv, octx, ictx, Ews, cp_default Ews d md nullval dsh dvals Ews c (Int.repr (ctx_size_of_MD (__EVP_MD DC))))
+         (OPENSSL_malloc_token 16 ictx * OPENSSL_malloc_token (ctx_size_of_MD (__EVP_MD DC)) md *
+           match_EVP_MD (__EVP_MD DC) dvals * OPENSSL_malloc_token 16 octx).
+  apply andp_right; auto.
+  - old_go_lower. entailer!.
+  - apply prop_right. simplify_Delta. Intros rv; Exists rv. old_go_lower.
+    Intros; subst. entailer!. rewrite sepcon_comm, distrib_orp_sepcon.
+    apply orp_left. 
+    * Intros. subst. rewrite if_true by trivial. Exists dsh dvals; entailer!.
+      unfold MDCTXHashed, MDCTXRaw, CTX_NULL, EVP_MD_CTX_NNnode.
+      Exists md. entailer!. unfold MD_state.
+      Exists c. rewrite C; simpl; entailer!.
+    * Intros buf; subst. rewrite if_false by discriminate. Exists dsh dvals; entailer!.
+      unfold MDCTXHashed, MDCTXRaw, CTX_NULL, EVP_MD_CTX_NNnode.
+      Exists buf md. entailer!. unfold MD_state.
+      Exists c c. rewrite C; simpl; entailer!.
++ (*Full*) clear H H0.
+  replace_SEP 0 (MDCTXFull D d ictx) by entailer!.
+  unfold MDCTXFull; Intros md.
+  replace_SEP 5 (MDCTXAllocated octx) by entailer!.
+  unfold MDCTXAllocated, CTX_NULL; Intros.
+  unfold EVP_of, EVP_MD_rep; Intros dsh dvals. rename H into Rsh; rename H0 into SZ.
+  rewrite data_at_isptr with (p:=d); Intros.
+  rewrite match_EVP_MD_getctxsize'; Intros; rename H into CTSZ.
+  unfold MD_state, data_block; Intros.
+  unfold postFin, MD_state. Intros finbytes. rename H into C(*; rename H0 into R*).
+  Exists (gv, octx, ictx, Ews, cp_default Ews d md nullval dsh dvals Ews finbytes (Int.repr (ctx_size_of_MD D)))
+         (OPENSSL_malloc_token 16 ictx * OPENSSL_malloc_token (ctx_size_of_MD D) md *
+           match_EVP_MD D dvals * OPENSSL_malloc_token 16 octx).
+  apply andp_right; auto.
+  - old_go_lower. entailer!.
+  - apply prop_right. simplify_Delta. Intros rv; Exists rv. old_go_lower.
+    Intros; subst. entailer!. rewrite sepcon_comm, distrib_orp_sepcon.
+    apply orp_left. 
+    * Intros. subst. rewrite if_true by trivial. Exists dsh dvals; entailer!.
+      unfold MDCTXFull, MDCTXRaw, CTX_NULL, EVP_MD_CTX_NNnode.
+      Exists md. entailer!. unfold postFin.
+      Exists finbytes. rewrite C; simpl; entailer!.
+    * Intros buf; subst. rewrite if_false by discriminate. Exists dsh dvals; entailer!.
+      unfold MDCTXFull, MDCTXRaw, CTX_NULL, EVP_MD_CTX_NNnode.
+      Exists buf md. entailer!. unfold postFin.
+      Exists finbytes finbytes. rewrite C; simpl; entailer!.
+Time Qed. (*3.5s*)
+
+Definition EVP_MD_CTX_copy_ex_ASPEC := DECLARE _EVP_MD_CTX_copy_ex
+  WITH gv:globals, octx:val, ictx:val, c: State
+  PRE [ _out OF (tptr (Tstruct _env_md_ctx_st noattr)),
+        _in OF (tptr (Tstruct _env_md_ctx_st noattr)) ]
+      PROP (c <> Allocated; c <> Raw)
+      LOCAL (gvars gv; temp _out octx; temp _in ictx)
+      SEP (MDCTX c ictx; EVP_of c; MDCTX Raw octx; mm_inv gv; ERRGV gv)
+  POST [ tint] EX rv:_,
+       PROP ()
+       LOCAL (temp ret_temp rv)
+       SEP (if Val.eq rv nullval then MDCTX Raw octx 
+            else (!!(rv=Vint Int.one) && MDCTX c octx);
+            ERRGV gv; mm_inv gv; MDCTX c ictx; EVP_of c).
+
+Lemma subsume_EVP_MD_CTX_copy_ex:
+      subsume_funspec (snd EVP_MD_CTX_copy_ex_SPEC) (snd EVP_MD_CTX_copy_ex_ASPEC).
+Proof.
+apply NDsubsume_subsume.
+{ split; reflexivity. }
+split3; auto.
+intros [[[gv octx] ictx] c]. specialize WA_WORD_nonneg; intros WAW.
+destruct c; Intros.
++ (*Allocated*) congruence.
++ (*Raw*) congruence.
++ (*Empty*) clear H H0.
+  replace_SEP 0 (MDCTXEmpty D d ictx) by entailer!.
+  unfold MDCTXEmpty; Intros md.
+  replace_SEP 5 (MDCTXRaw octx) by entailer!.
+  unfold MDCTXRaw, CTX_NULL; Intros.
+  unfold EVP_of, EVP_MD_rep; Intros dsh dvals. rename H into Rsh; rename H0 into SZ.
+  rewrite data_at_isptr with (p:=d); Intros.
+  rewrite match_EVP_MD_getctxsize'; Intros; rename H into CTSZ.
+  unfold MD_state, data_block; Intros c. rename H into C. rename H0 into SZmod. rename H1 into HR.
+  Exists (gv, octx, ictx, copyEx_other Ews d md nullval nullval dsh dvals Ews nullval nullval nullval
+                           (Int.repr (ctx_size_of_MD D)) Ews c None)
+          (match_EVP_MD D dvals * OPENSSL_malloc_token 16 ictx * 
+           OPENSSL_malloc_token 16 octx * OPENSSL_malloc_token (ctx_size_of_MD D) md).
+  apply andp_right; auto.
+  - old_go_lower.
+    rewrite if_false. 2: destruct d; try contradiction; discriminate.
+    entailer!.
+  - apply prop_right. simplify_Delta. Intros rv; Exists rv. old_go_lower.
+    rewrite if_false. 2: destruct d; try contradiction; discriminate.
+    Exists dsh dvals.
+    Intros; subst. entailer!. rewrite sepcon_comm, distrib_orp_sepcon.
+    apply orp_left. 
+    * Intros. subst. rewrite if_true by trivial. cancel. 
+      unfold MDCTXEmpty, MDCTXRaw, CTX_NULL, EVP_MD_CTX_NNnode, match_EVP_MD.
+      Exists md. entailer!. unfold MD_state.
+      Exists c. rewrite C; simpl; entailer!.
+    * Intros buf; subst. rewrite if_false by discriminate.
+      unfold MDCTXEmpty, MDCTXRaw, CTX_NULL, EVP_MD_CTX_NNnode, match_EVP_MD.
+      Exists buf md. entailer!. unfold MD_state.
+      Exists c c. rewrite C; simpl; entailer!.
++ (*Hashed*) clear H H0.
+  replace_SEP 0 (MDCTXHashed DC d ictx) by entailer!.
+  unfold MDCTXHashed; Intros md.
+  replace_SEP 5 (MDCTXRaw octx) by entailer!.
+  unfold MDCTXRaw, CTX_NULL; Intros.
+  unfold EVP_of, EVP_MD_rep; Intros dsh dvals. rename H into Rsh; rename H0 into SZ.
+  rewrite data_at_isptr with (p:=d); Intros.
+  rewrite match_EVP_MD_getctxsize'; Intros; rename H into CTSZ.
+  unfold MD_state, data_block; Intros c. rename H into C.
+  Exists (gv, octx, ictx, copyEx_other Ews d md nullval nullval dsh dvals Ews nullval nullval nullval
+                           (Int.repr (ctx_size_of_MD (__EVP_MD DC))) Ews c None)
+          (match_EVP_MD (__EVP_MD DC) dvals * OPENSSL_malloc_token 16 ictx * 
+           OPENSSL_malloc_token 16 octx * OPENSSL_malloc_token (ctx_size_of_MD (__EVP_MD DC)) md).
+  apply andp_right; auto.
+  - old_go_lower.
+    rewrite if_false. 2: destruct d; try contradiction; discriminate.
+    entailer!.
+  - apply prop_right. simplify_Delta. Intros rv; Exists rv. old_go_lower.
+    rewrite if_false. 2: destruct d; try contradiction; discriminate.
+    Exists dsh dvals.
+    Intros; subst. entailer!. rewrite sepcon_comm, distrib_orp_sepcon.
+    apply orp_left. 
+    * Intros. subst. rewrite if_true by trivial. cancel.
+      unfold MDCTXHashed, MDCTXRaw, CTX_NULL, EVP_MD_CTX_NNnode, match_EVP_MD.
+      Exists md. entailer!. unfold MD_state.
+      Exists c. rewrite C; simpl; entailer!.
+    * Intros buf; subst. rewrite if_false by discriminate.
+      unfold MDCTXHashed, MDCTXRaw, CTX_NULL, EVP_MD_CTX_NNnode, match_EVP_MD.
+      Exists buf md. entailer!. unfold MD_state.
+      Exists c c. rewrite C; simpl; entailer!.
++ (*Full*) clear H H0.
+  replace_SEP 0 (MDCTXFull D d ictx) by entailer!.
+  unfold MDCTXFull; Intros md.
+  replace_SEP 5 (MDCTXRaw octx) by entailer!.
+  unfold MDCTXRaw, CTX_NULL; Intros.
+  unfold EVP_of, EVP_MD_rep; Intros dsh dvals. rename H into Rsh; rename H0 into SZ.
+  rewrite data_at_isptr with (p:=d); Intros.
+  rewrite match_EVP_MD_getctxsize'; Intros; rename H into CTSZ.
+  unfold MD_state, data_block; Intros.
+  unfold postFin, MD_state. Intros finbytes. rename H into C(*; rename H0 into R*).
+  Exists (gv, octx, ictx, copyEx_other Ews d md nullval nullval dsh dvals Ews nullval nullval nullval
+                           (Int.repr (ctx_size_of_MD D)) Ews finbytes None)
+          (match_EVP_MD D dvals * OPENSSL_malloc_token 16 ictx * 
+           OPENSSL_malloc_token 16 octx * OPENSSL_malloc_token (ctx_size_of_MD D) md).
+  apply andp_right; auto.
+  - old_go_lower.
+    rewrite if_false. 2: destruct d; try contradiction; discriminate.
+    (*rewrite H4; simpl.*) entailer!.
+  - apply prop_right. simplify_Delta. Intros rv; Exists rv. old_go_lower.
+    rewrite if_false. 2: destruct d; try contradiction; discriminate.
+    Exists dsh dvals.
+    Intros; subst. entailer!. rewrite sepcon_comm, distrib_orp_sepcon.
+    apply orp_left. 
+    * Intros. subst. rewrite if_true by trivial. cancel.
+      unfold MDCTXFull, MDCTXRaw, CTX_NULL, EVP_MD_CTX_NNnode, match_EVP_MD.
+      Exists md. entailer!. unfold postFin, MD_state. Exists finbytes.
+      rewrite C; simpl; entailer!.
+    * Intros buf; subst. rewrite if_false by discriminate.
+      unfold MDCTXFull, MDCTXRaw, CTX_NULL, EVP_MD_CTX_NNnode, match_EVP_MD.
+      Exists buf md. entailer!. unfold postFin, MD_state. Exists finbytes finbytes.
+      rewrite C; simpl; entailer!. 
+Time Qed. (*3.5s*)
+
+Definition EVP_MD_CTX_newcreate_ASPEC :=
+   WITH gv:globals
+   PRE [ ]
+       PROP (24 <= Int.max_unsigned - (WA + WORD))
+       LOCAL (gvars gv)
+       SEP (mm_inv gv)
+   POST [ tptr (Tstruct _env_md_ctx_st noattr) ]
+     EX ctx:val,
+       PROP ()
+       LOCAL (temp ret_temp ctx)
+       SEP ((!!(ctx=nullval) && emp) || MDCTX Raw ctx; mm_inv gv).
+
+Definition EVP_MD_CTX_create_ASPEC := DECLARE _EVP_MD_CTX_create EVP_MD_CTX_newcreate_ASPEC.
+Definition EVP_MD_CTX_new_ASPEC := DECLARE _EVP_MD_CTX_new EVP_MD_CTX_newcreate_ASPEC.
+
+Definition EVP_DigestUpdate_ASPEC := DECLARE _EVP_DigestUpdate
+  WITH ctx: val, t:val, d: val, dsh:share, data: list byte, DC: MD_with_content, len:Z
+  PRE [ _ctx OF tptr (Tstruct _env_md_ctx_st noattr), _data OF tptr tvoid,  _len OF tuint ]
+      PROP (readable_share dsh; UpdateSideconditions DC data len)
+      LOCAL (temp _ctx ctx; temp _data d; temp _len (Vint (Int.repr len)) )
+      SEP (MDCTX (Hashed DC t) ctx; data_block dsh data d; EVP_MD_rep (__EVP_MD DC) t)
+  POST [ tint] 
+       PROP ()
+       LOCAL (temp ret_temp (Vint Int.one))
+       SEP (MDCTX (Hashed (UPD DC data len) t) ctx; data_block dsh data d; EVP_MD_rep (__EVP_MD DC) t).
+
+Definition EVP_MD_CTX_freedestroy_ASPEC :=
+  WITH gv:globals, ctx:val, c: State
+  PRE [ _ctx OF (tptr (Tstruct _env_md_ctx_st noattr)) ]
+      PROP (c <> Allocated)
+      LOCAL (gvars gv; temp _ctx ctx)
+      SEP (MDCTX c ctx; mm_inv gv)
+  POST [ tvoid ]
+       PROP ()
+       LOCAL ()
+       SEP (mm_inv gv).
+
+Definition EVP_MD_CTX_free_ASPEC := DECLARE _EVP_MD_CTX_free EVP_MD_CTX_freedestroy_ASPEC.
+Definition EVP_MD_CTX_destroy_ASPEC := DECLARE _EVP_MD_CTX_destroy EVP_MD_CTX_freedestroy_ASPEC.
+
+Definition EVP_MD_CTX_cleanupreset_ASPEC :=
+  WITH gv:globals, ctx:val, c: State
+  PRE [ _ctx OF (tptr (Tstruct _env_md_ctx_st noattr)) ]
+      PROP (c <> Allocated) LOCAL (gvars gv; temp _ctx ctx)
+      SEP (MDCTX c ctx; EVP_of c; mm_inv gv)
+  POST [ tint ]
+       PROP () LOCAL (temp ret_temp (Vint (Int.one)))
+       SEP (MDCTX Raw ctx; EVP_of c; mm_inv gv).
+
+Definition EVP_MD_CTX_cleanup_ASPEC := DECLARE _EVP_MD_CTX_cleanup EVP_MD_CTX_cleanupreset_ASPEC.
+
+(*Note that this is the same spec as cleanup! Indeed the comment in the header file
+  suggests that the precondition should be that of cleanup, whereas the fact that
+  cleanup results in an initialized (not merely allocated) ctx means that doing
+  init again does not change much*)
+Definition EVP_MD_CTX_reset_ASPEC := DECLARE _EVP_MD_CTX_reset EVP_MD_CTX_cleanupreset_ASPEC.
+
+Definition EVP_DigestFinal_ex_ASPEC := DECLARE _EVP_DigestFinal_ex
+  WITH ctx: val, t:val, 
+       out: val, osh:share, sz:val,
+       DC:MD_with_content
+  PRE [ _ctx OF tptr (Tstruct _env_md_ctx_st noattr),
+        _md_out OF tptr tuchar, _size OF tptr tuint]
+      PROP (writable_share osh;
+            0 <= ctx_size_of_MD (__EVP_MD DC) <= Int.max_unsigned)
+      LOCAL (temp _ctx ctx; temp _md_out out; temp _size sz)
+      SEP (MDCTX (Hashed DC t) ctx; EVP_MD_rep (__EVP_MD DC) t;
+           if Val.eq sz nullval then emp else data_at_ Ews tuint sz;
+           memory_block osh (md_size_of_MD (__EVP_MD DC)) out)
+  POST [ tint] 
+       PROP ()
+       LOCAL (temp ret_temp (Vint Int.one))
+       SEP (MDCTX (Full (__EVP_MD DC) t) ctx; EVP_MD_rep (__EVP_MD DC) t;
+            if Val.eq sz nullval then emp else data_at Ews tuint (Vint (Int.repr (md_size_of_MD (__EVP_MD DC)))) sz;
+            data_block osh (FIN DC) out).
+
+Definition EVP_DigestFinal_ASPEC := DECLARE _EVP_DigestFinal
+  WITH gv: globals, ctx: val, t:val, 
+       out: val, osh:share, sz:val,
+       DC:MD_with_content
+  PRE [_ctx OF tptr (Tstruct _env_md_ctx_st noattr),
+        _md OF tptr tuchar, _size OF tptr tuint]
+      PROP (writable_share osh;
+            0 <= ctx_size_of_MD (__EVP_MD DC) <= Int.max_unsigned)
+      LOCAL (gvars gv; temp _ctx ctx; temp _md out; temp _size sz )
+      SEP (MDCTX (Hashed DC t) ctx; EVP_MD_rep (__EVP_MD DC) t;
+           if Val.eq sz nullval then emp else data_at_ Ews tuint sz;
+           memory_block osh (md_size_of_MD (__EVP_MD DC)) out; mm_inv gv)
+  POST [ tint] 
+       PROP ()
+       LOCAL (temp ret_temp (Vint Int.one))
+       SEP (MDCTX Raw ctx;
+            EVP_MD_rep (__EVP_MD DC) t;
+            if Val.eq sz nullval then emp else data_at Ews tuint (Vint (Int.repr (md_size_of_MD (__EVP_MD DC)))) sz;
+            data_block osh (FIN DC) out; mm_inv gv).
+
+Definition EVP_DigestInitExPre T t c ctx :=
+  match c with
+| Allocated => FF
+| Raw => MDCTX c ctx * EVP_MD_rep T t
+| Empty D d => MDCTX c ctx * EVP_MD_rep T t * if Val.eq d t then !!(D=T) && emp else (!!(D<>T) && EVP_MD_rep D d)
+| Hashed DC d => MDCTX c ctx * EVP_MD_rep T t * 
+                 let D := __EVP_MD DC in
+                 if Val.eq d t then !!(D=T) && emp else (!!(D<>T) && EVP_MD_rep D d)
+| Full D d => MDCTX c ctx * EVP_MD_rep T t * if Val.eq d t then !!(D=T) && emp else (!!(D<>T) && EVP_MD_rep D d)
+  end.
+
+Definition EVP_DigestInitExPost T t c rv ctx :=
+  match c with
+  Allocated => FF
+| Raw => if Val.eq rv nullval then MDCTX c ctx else
+         !!(rv=Vint Int.one) && MDCTX (Empty T t) ctx
+| Empty D d => if Val.eq rv nullval 
+                 then !!(d<>t) && MDCTX c ctx * EVP_MD_rep D d
+                 else (!!(rv=Vint Int.one) && MDCTX (Empty T t) ctx * if Val.eq d t then emp else EVP_MD_rep D d)
+| Hashed DC d => if Val.eq rv nullval 
+                 then !!(d<>t) && MDCTX c ctx * EVP_MD_rep (__EVP_MD DC) d
+                 else (!!(rv=Vint Int.one) && MDCTX (Empty T t) ctx * if Val.eq d t then emp else EVP_MD_rep (__EVP_MD DC) d)
+| Full D d => if Val.eq rv nullval 
+                 then !!(d<>t) && MDCTX c ctx * EVP_MD_rep D d
+                 else (!!(rv=Vint Int.one) && MDCTX (Empty T t) ctx * if Val.eq d t then emp else EVP_MD_rep D d)
+  end.
+
+(*Header file specifies that ictx must already be initialized, ie Allocated state is ruled out*)
+Definition EVP_DigestInit_ex_ASPEC := DECLARE _EVP_DigestInit_ex
+  WITH gv:globals, ctx:val, t:val, e:val, T: EVP_MD, c: State
+  PRE [ _ctx OF tptr (Tstruct _env_md_ctx_st noattr), 
+        _type OF tptr (Tstruct _env_md_st noattr),
+        _engine OF tptr (Tstruct _engine_st noattr) ]
+      PROP (4 <= ctx_size_of_MD T <= Int.max_unsigned - (WA + WORD) - 8; c <> Allocated)
+      LOCAL (gvars gv; temp _type t; temp _ctx ctx; temp _engine e)
+      SEP (EVP_DigestInitExPre T t c ctx; ERRGV gv; mm_inv gv)
+  POST [ tint] EX rv:_,
+       PROP ()
+       LOCAL (temp ret_temp rv)
+       SEP (EVP_DigestInitExPost T t c rv ctx;ERRGV gv; EVP_MD_rep T t; mm_inv gv).
+
+(*
+Definition EVP_DigestInit_ASPEC := DECLARE _EVP_DigestInit
+  WITH gv:globals, ctx:val, t:val, T: EVP_MD, c: State
+  PRE [ _ctx OF tptr (Tstruct _env_md_ctx_st noattr), 
+        _type OF tptr (Tstruct _env_md_st noattr) ]
+      PROP (4 <= ctx_size_of_MD T <= Int.max_unsigned - (WA + WORD) - 8)
+      LOCAL (gvars gv; temp _type t; temp _ctx ctx)
+      SEP (MDCTX c ctx; EVP_MD_rep T t; ERRGV gv; mm_inv gv)
+  POST [ tint] EX rv:_,
+       PROP ()
+       LOCAL (temp ret_temp rv)
+       SEP (if Val.eq rv nullval  then MDCTX Raw ctx
+            else !!(rv=Vint Int.one) && MDCTX (Empty T t) ctx;
+            LEAK c; ERRGV gv; EVP_MD_rep T t; mm_inv gv).*)
+Definition EVP_DigestInit_ASPEC := DECLARE _EVP_DigestInit
+  WITH gv:globals, ctx:val, t:val, T: EVP_MD
+  PRE [ _ctx OF tptr (Tstruct _env_md_ctx_st noattr), 
+        _type OF tptr (Tstruct _env_md_st noattr) ]
+      PROP (4 <= ctx_size_of_MD T <= Int.max_unsigned - (WA + WORD) - 8)
+      LOCAL (gvars gv; temp _type t; temp _ctx ctx)
+      SEP (MDCTX Allocated ctx; EVP_MD_rep T t; ERRGV gv; mm_inv gv)
+  POST [ tint] EX rv:_,
+       PROP ()
+       LOCAL (temp ret_temp rv)
+       SEP (if Val.eq rv nullval then MDCTX Raw ctx
+            else !!(rv=Vint Int.one) && MDCTX (Empty T t) ctx;
+            ERRGV gv; EVP_MD_rep T t; mm_inv gv).
+
+Lemma subsume_EVP_MD_CTX_cleanupreset:
+      subsume_funspec EVP_MD_CTX_cleanupreset_SPEC EVP_MD_CTX_cleanupreset_ASPEC.
+Proof.
+apply NDsubsume_subsume.
+{ split; reflexivity. }
+split3; auto.
+intros [[gv ctx] c]. destruct c.
++ (*Allocated*) Intros; congruence.
++ (*Raw*) Intros; clear H.
+  Exists (gv, ctx, Ews, nullval, @None Z) (OPENSSL_malloc_token 16 ctx).
+  apply andp_right; auto.
+  - old_go_lower. unfold MDCTXRaw, CTX_NULL. entailer!.
+    Exists nullval nullval. entailer!. 
+  - apply prop_right. simplify_Delta. old_go_lower; unfold MDCTXRaw, CTX_NULL; entailer!.
++ (*Empty*) Intros; clear H.
+  replace_SEP 0 (MDCTXEmpty D d ctx) by entailer!.
+  unfold MDCTXEmpty; Intros md.
+  Exists (gv, ctx, Ews, md, Some (ctx_size_of_MD D)) (EVP_MD_rep D d * OPENSSL_malloc_token 16 ctx).
+  apply andp_right; auto.
+  - old_go_lower. Exists d nullval. entailer!. apply MD_state_memoryblock.
+  - apply prop_right. simplify_Delta. old_go_lower; unfold MDCTXRaw; entailer!.
++ (*Hashed*) Intros; clear H.
+  replace_SEP 0 (MDCTXHashed DC d ctx) by entailer!.
+  unfold MDCTXHashed; Intros md. destruct DC as [D data].
+  Exists (gv, ctx, Ews, md, Some (ctx_size_of_MD D)) (EVP_MD_rep D d * OPENSSL_malloc_token 16 ctx).
+  apply andp_right; auto.
+  - old_go_lower. Exists d nullval. entailer!. apply MD_state_memoryblock.
+  - apply prop_right. simplify_Delta. old_go_lower; unfold MDCTXRaw; entailer!.
++ (*Full*) Intros; clear H.
+  replace_SEP 0 (MDCTXFull D d ctx) by entailer!.
+  unfold MDCTXFull; Intros md.
+  Exists (gv, ctx, Ews, md, Some (ctx_size_of_MD D)) (EVP_MD_rep D d * OPENSSL_malloc_token 16 ctx).
+  apply andp_right; auto.
+  - old_go_lower. Exists d nullval. entailer!. apply postFin_memory_block. (*apply MD_state_memoryblock.*)
+  - apply prop_right. simplify_Delta. old_go_lower; unfold MDCTXRaw; entailer!.
+Qed.
+
+Lemma subsume_EVP_MD_CTX_newcreate:
+      subsume_funspec EVP_MD_CTX_newcreate_SPEC EVP_MD_CTX_newcreate_ASPEC.
+Proof.
+apply NDsubsume_subsume.
+{ split; reflexivity. }
+split3; auto.
+intros gv. Exists gv emp.
+change (`emp) with (@emp (environ->mpred) _ _); rewrite !emp_sepcon.
+apply andp_right; auto.
++ entailer!. 
++ apply prop_right. simplify_Delta. Intros ctx. Exists ctx. entailer.
+Qed.
+
+(*Identical proof to subsume_EVP_MD_CTX_new*)
+Lemma subsume_EVP_MD_CTX_create:
+      subsume_funspec (snd EVP_MD_CTX_create_SPEC) (snd EVP_MD_CTX_create_ASPEC).
+Proof.
+apply NDsubsume_subsume.
+{ split; reflexivity. }
+split3; auto.
+intros gv. Exists gv emp.
+change (`emp) with (@emp (environ->mpred) _ _); rewrite !emp_sepcon.
+apply andp_right; auto.
++ entailer!. 
++ apply prop_right. simplify_Delta. Intros ctx. Exists ctx. entailer.
+Qed.
+
+Lemma subsume_EVP_DigestUpdate:
+      subsume_funspec (snd EVP_DigestUpdate_SPEC) (snd EVP_DigestUpdate_ASPEC).
+Proof.
+apply NDsubsume_subsume.
+{ split; reflexivity. }
+split3; auto.
+intros [[[[[[ctx t] d] dsh] data] DC] len]. 
+rewrite EVP_MD_rep_isptr'; Intros. rename H into Rdsh. rename H0 into SC.
+replace_SEP 0 (MDCTXHashed DC t ctx) by entailer!.
+unfold MDCTXHashed, EVP_MD_CTX_NNnode; Intros md.
+Exists (ctx, Ews, (t, (md, (nullval, nullval))), d, dsh, data, DC, len, Ews)
+       (OPENSSL_malloc_token (ctx_size_of_MD (__EVP_MD DC)) md * OPENSSL_malloc_token 16 ctx).
+apply andp_right.
++ old_go_lower; entailer!.
++ apply prop_right. simplify_Delta. old_go_lower; entailer.
+  unfold MDCTXHashed, EVP_MD_CTX_NNnode; simpl.
+  Exists md. entailer!.
+Qed.
+
+Lemma subsume_EVP_MD_CTX_freedestroy:
+      subsume_funspec EVP_MD_CTX_freedestroy_SPEC EVP_MD_CTX_freedestroy_ASPEC.
+Proof.
+apply NDsubsume_subsume.
+{ split; reflexivity. }
+split3; auto.
+intros [[gv ctx] c]. destruct c.
++ (*Allocated*) Intros; congruence.
++ (*Raw*) Intros; clear H. 
+  replace_SEP 0 (MDCTXRaw ctx) by entailer!.
+  Exists (gv, ctx, nullval, nullval, nullval, @None Z) emp.
+  change (`emp) with (@emp (environ->mpred) _ _); rewrite !emp_sepcon.
+  apply andp_right; auto.
+  - entailer!. apply orp_right2. unfold MDCTXRaw, CTX_NULL; entailer!.
+  - entailer!.
++ (*Empty*) Intros; clear H.
+  replace_SEP 0 (MDCTXEmpty D d ctx) by entailer!.
+  unfold MDCTXEmpty. Intros md.
+  Exists (gv, ctx, d, md, nullval, Some (ctx_size_of_MD D)) emp.
+  change (`emp) with (@emp (environ->mpred) _ _); rewrite !emp_sepcon.
+  apply andp_right; auto.
+  - entailer!. apply orp_right2. entailer!. apply MD_state_memoryblock. 
+  - apply prop_right. simplify_Delta. entailer!. 
++ (*Hashed*) Intros; clear H. 
+  replace_SEP 0 (MDCTXHashed DC d ctx) by entailer!.
+  unfold MDCTXHashed. Intros md.
+  Exists (gv, ctx, d, md, nullval, Some (ctx_size_of_MD (__EVP_MD DC))) emp.
+  change (`emp) with (@emp (environ->mpred) _ _); rewrite !emp_sepcon.
+  apply andp_right; auto.
+  - Time entailer!. simpl in *. apply orp_right2. entailer!. apply MD_state_memoryblock.
+  - apply prop_right. simplify_Delta. entailer!. 
++ (*Full*) Intros; clear H. 
+  replace_SEP 0 (MDCTXFull D d ctx) by entailer!.
+  unfold MDCTXFull. Intros md.
+  Exists (gv, ctx, d, md, nullval, Some (ctx_size_of_MD D)) emp.
+  change (`emp) with (@emp (environ->mpred) _ _); rewrite !emp_sepcon.
+  apply andp_right; auto. 
+  - go_lower; simpl in *. cancel. apply andp_right. apply prop_right; intuition.
+    cancel. apply orp_right2. cancel. apply postFin_memory_block.
+  - apply prop_right. simplify_Delta. entailer!. 
+Qed.
+
+Lemma subsume_EVP_DigestFinal_ex:
+      subsume_funspec (snd EVP_DigestFinal_ex_SPEC) (snd EVP_DigestFinal_ex_ASPEC).
+Proof.
+apply NDsubsume_subsume.
+{ split; reflexivity. }
+split3; auto.
+intros [[[[[ctx t] out] osh] sz] DC].
+rewrite EVP_MD_rep_isptr'; Intros. rename H into Wosh. rename H0 into SZ.
+replace_SEP 0 (MDCTXHashed DC t ctx) by entailer!.
+unfold MDCTXHashed, EVP_MD_CTX_NNnode; Intros md.
+Exists (ctx, Ews, (t, (md, (nullval, nullval))), out, osh, sz, DC, Ews)
+       (OPENSSL_malloc_token (ctx_size_of_MD (__EVP_MD DC)) md * OPENSSL_malloc_token 16 ctx).
+apply andp_right.
++ old_go_lower; entailer!.
++ apply prop_right. simplify_Delta. old_go_lower. Time entailer!.
+  Exists md. cancel. apply sepcon_derives; [unfold EVP_MD_CTX_NNnode; entailer! | apply derives_refl].
+Qed.
+
+Lemma subsume_EVP_DigestFinal:
+      subsume_funspec (snd EVP_DigestFinal_SPEC) (snd EVP_DigestFinal_ASPEC).
+Proof.
+apply NDsubsume_subsume.
+{ split; reflexivity. }
+split3; auto.
+intros [[[[[[gv ctx] t] out] osh] sz] DC].
+rewrite EVP_MD_rep_isptr'; Intros. rename H into Wosh. rename H0 into SZ.
+replace_SEP 0 (MDCTXHashed DC t ctx) by entailer!.
+unfold MDCTXHashed, EVP_MD_CTX_NNnode; Intros md.
+Exists (gv, ctx, Ews, (t, (md, (nullval, nullval))), out, osh, sz, DC)
+       (OPENSSL_malloc_token 16 ctx).
+apply andp_right.
++ old_go_lower; entailer!.
++ apply prop_right. simplify_Delta. old_go_lower; entailer!.
+  unfold MDCTXRaw; cancel. 
+Qed.
+
+Lemma subsume_EVP_DigestInit_ex:
+      subsume_funspec (snd EVP_DigestInit_ex_SPEC) (snd EVP_DigestInit_ex_ASPEC).
+Proof.
+apply NDsubsume_subsume.
+{ split; reflexivity. }
+split3; auto.
+intros [[[[[gv ctx] t] e] T] c]. rewrite EVP_MD_rep_isptr'; Intros. rename H into SCT.
+specialize WA_WORD_nonneg; intros WAW. 
+destruct c; [ congruence | | | |]; clear H0.
++ (*Raw*)
+  replace_SEP 0 (MDCTXRaw ctx * EVP_MD_rep T t) by entailer!.
+  unfold MDCTXRaw.
+  rewrite OPENSSL_malloc_token_compatible', EVP_MD_rep_isptr'; Intros.
+  Exists (ctx, t, e, nullval, nullval, (nullval, nullval), T, gv, Ews, DIEC_NEQ None None)
+         (OPENSSL_malloc_token 16 ctx).
+  apply andp_right; auto.
+  - old_go_lower. entailer!.
+    unfold CTX_NULL; cancel.
+  - apply prop_right. Intros rv. Exists rv. simplify_Delta. unfold DIE_postMpred.
+    old_go_lower; entailer; cancel.
+    rewrite sepcon_comm, distrib_orp_sepcon. apply orp_left.
+    * Intros; subst. rewrite if_true; trivial. unfold MDCTXRaw, CTX_NULL; cancel.
+    * Intros m; subst; rewrite if_false by discriminate.
+      rewrite OPENSSL_malloc_token_compatible'; Intros.
+      entailer!. unfold MDCTXEmpty, EVP_MD_CTX_NNnode.
+      Exists m; entailer!.
++ (*Empty*)
+  replace_SEP 0 (MDCTXEmpty D d ctx * EVP_MD_rep T t *
+      (if Val.eq d t then !! (D = T) && emp else !! (D <> T) && EVP_MD_rep D d)) by entailer!.
+  unfold MDCTXEmpty. Intros m.
+  rewrite OPENSSL_malloc_token_compatible' with (v:=m), EVP_MD_rep_isptr' with (p:=t); Intros.
+  rename H0 into SZD; rename H into MCm.
+  destruct (Val.eq d t); Intros; subst.
+  * (*d=t, D=T*)
+    Exists (ctx, t, e, t, m, (nullval, nullval), T, gv, Ews, DIEC_EQ)
+           (OPENSSL_malloc_token 16 ctx * mm_inv gv * OPENSSL_malloc_token (ctx_size_of_MD T) m).
+    apply andp_right; auto.
+    - old_go_lower. entailer. cancel. 
+      eapply derives_trans. apply MD_state_memoryblock. simpl. apply preInit_fresh_EWS; rep_omega.
+    - apply prop_right. Intros rv. Exists rv. simplify_Delta. unfold DIE_postMpred.
+      old_go_lower; entailer!. rewrite if_false by discriminate. rewrite if_true by trivial.
+      unfold MDCTXEmpty. Exists m. entailer!. 
+      unfold EVP_MD_CTX_NNnode. entailer!.
+  * (*d<>t, D<>T*)
+    rewrite EVP_MD_rep_isptr' with (p:=d); Intros.
+    unfold EVP_MD_rep at 2. Intros dsh dvals.
+    unfold MD_state. Intros bytes. 
+    Exists (ctx, t, e, d, m, (nullval, nullval), T, gv, Ews, DIEC_NEQ (Some (dsh,dvals)) 
+            (Some (*(INI D)*)(D, bytes)))
+           (OPENSSL_malloc_token 16 ctx * match_EVP_MD D dvals).
+    apply andp_right; auto.
+    - old_go_lower. entailer. cancel. unfold EVP_MD_NNnode. entailer!. 
+    - apply prop_right. Intros rv. Exists rv. simplify_Delta. unfold DIE_postMpred.
+      old_go_lower; simpl; entailer!. 
+      rewrite sepcon_assoc. rewrite sepcon_comm, ! distrib_orp_sepcon. apply orp_left.
+      { Intros; subst. rewrite if_true by trivial. 
+        unfold MDCTXEmpty, EVP_MD_CTX_NNnode. Exists m; entailer. cancel.
+        unfold EVP_MD_rep, EVP_MD_NNnode. Exists dsh dvals. entailer!.
+         unfold MD_state. Exists bytes. rewrite H2; simpl; entailer!. }
+      { Intros md; subst. rewrite if_false by discriminate.
+        rewrite OPENSSL_malloc_token_compatible' with (v:=md).
+        unfold MDCTXEmpty, EVP_MD_CTX_NNnode. Exists md; entailer. cancel.
+        rewrite if_false by trivial.
+        unfold EVP_MD_rep, EVP_MD_NNnode. Exists dsh dvals. entailer!.  }
++ (*Hashed*)
+  replace_SEP 0 (MDCTXHashed DC d ctx * EVP_MD_rep T t *
+      (if Val.eq d t then !! (__EVP_MD DC = T) && emp else !! (__EVP_MD DC <> T) && EVP_MD_rep (__EVP_MD DC) d)) by entailer!.
+  unfold MDCTXHashed. Intros m.
+  rewrite OPENSSL_malloc_token_compatible' with (v:=m), EVP_MD_rep_isptr' with (p:=t); Intros.
+  rename H0 into SZD; rename H into MCm.
+  destruct (Val.eq d t); Intros; subst.
+  * (*d=t, D=T*)
+    Exists (ctx, t, e, t, m, (nullval, nullval), __EVP_MD DC, gv, Ews, DIEC_EQ)
+           (OPENSSL_malloc_token 16 ctx * mm_inv gv * OPENSSL_malloc_token (ctx_size_of_MD (__EVP_MD DC)) m).
+    apply andp_right; auto.
+    - old_go_lower. entailer. cancel.
+      eapply derives_trans. apply MD_state_memoryblock. simpl. apply preInit_fresh_EWS; rep_omega.
+    - apply prop_right. Intros rv. Exists rv. simplify_Delta. unfold DIE_postMpred.
+      old_go_lower; entailer!. rewrite if_false by discriminate. rewrite if_true by trivial.
+      unfold MDCTXEmpty. Exists m. entailer!. 
+      unfold EVP_MD_CTX_NNnode. entailer!.
+  * (*d<>t, D<>T*)
+    rewrite EVP_MD_rep_isptr' with (p:=d); Intros.
+    unfold EVP_MD_rep at 2. Intros dsh dvals.
+    unfold MD_state; Intros bytes.
+    Exists (ctx, t, e, d, m, (nullval, nullval), T, gv, Ews, 
+            DIEC_NEQ (Some (dsh,dvals)) (Some (__EVP_MD DC,bytes)))
+           (OPENSSL_malloc_token 16 ctx * match_EVP_MD (__EVP_MD DC) dvals).
+    apply andp_right; auto.
+    - old_go_lower. entailer. cancel. unfold EVP_MD_NNnode. entailer!.
+    - apply prop_right. Intros rv. Exists rv. simplify_Delta. unfold DIE_postMpred.
+      old_go_lower; simpl; entailer!. 
+      rewrite sepcon_assoc. rewrite sepcon_comm, ! distrib_orp_sepcon. apply orp_left.
+      { Intros; subst. rewrite if_true by trivial. 
+        unfold MDCTXHashed, EVP_MD_CTX_NNnode. Exists m; entailer. cancel.
+        unfold EVP_MD_rep, EVP_MD_NNnode. Exists dsh dvals. entailer!.
+        unfold MD_state, data_block. Exists bytes. rewrite H2; simpl; entailer!. }
+      { Intros md; subst. rewrite if_false by discriminate.
+        rewrite OPENSSL_malloc_token_compatible' with (v:=md).
+        unfold MDCTXEmpty, EVP_MD_CTX_NNnode. Exists md; entailer. cancel.
+        rewrite if_false by trivial.
+        unfold EVP_MD_rep, EVP_MD_NNnode. Exists dsh dvals. entailer!. }
++ (*Full*)
+  replace_SEP 0 (MDCTXFull D d ctx * EVP_MD_rep T t *
+      (if Val.eq d t then !! (D = T) && emp else !! (D <> T) && EVP_MD_rep D d)) by entailer!.
+  unfold MDCTXFull. Intros m.
+  rewrite OPENSSL_malloc_token_compatible' with (v:=m), EVP_MD_rep_isptr' with (p:=t); Intros.
+  rename H0 into SZD; rename H into MCm.
+  unfold postFin; Intros findata.
+(*  rewrite (PF D m).*)
+  destruct (Val.eq d t); Intros; subst.
+  * (*d=t, D=T*)
+    Exists (ctx, t, e, t, m, (nullval, nullval), T, gv, Ews, DIEC_EQ)
+           (OPENSSL_malloc_token 16 ctx * mm_inv gv * OPENSSL_malloc_token (ctx_size_of_MD T) m).
+    apply andp_right; auto.
+    - old_go_lower. entailer. cancel. unfold preInit. rewrite <- H; entailer!.
+       sep_apply (data_at_memory_block Ews (__type findata) (__values findata) m).
+       rewrite memory_block_data_at__tarray_tuchar_eq; trivial. omega. 
+    - apply prop_right. Intros rv. Exists rv. simplify_Delta. unfold DIE_postMpred.
+      old_go_lower; entailer!. rewrite if_false by discriminate. rewrite if_true by trivial.
+      unfold MDCTXEmpty. Exists m. entailer!. 
+      unfold EVP_MD_CTX_NNnode. entailer!.
+  * (*d<>t, D<>T*)
+    rewrite EVP_MD_rep_isptr' with (p:=d); Intros.
+    unfold EVP_MD_rep at 2. Intros dsh dvals.
+    Exists (ctx, t, e, d, m, (nullval, nullval), T, gv, Ews, 
+            DIEC_NEQ (Some (dsh,dvals)) (Some (D, findata) (*({| __EVP_MD := D; __content := findata |})*)))
+           (OPENSSL_malloc_token 16 ctx * match_EVP_MD D dvals).
+    apply andp_right; auto.
+    - old_go_lower. entailer. cancel. unfold EVP_MD_NNnode. entailer!.
+    - apply prop_right. Intros rv. Exists rv. simplify_Delta. unfold DIE_postMpred.
+      old_go_lower; simpl; entailer!.
+      rewrite sepcon_assoc. rewrite sepcon_comm, ! distrib_orp_sepcon. apply orp_left.
+      { Intros; subst. rewrite if_true by trivial. 
+        unfold MDCTXFull, EVP_MD_CTX_NNnode. Exists m; entailer. cancel.
+        unfold EVP_MD_rep, EVP_MD_NNnode. Exists dsh dvals. entailer!.
+        unfold postFin, data_block. Exists findata; rewrite H; simpl. entailer!. }
+      { Intros md; subst. rewrite if_false by discriminate.
+        rewrite OPENSSL_malloc_token_compatible' with (v:=md).
+        unfold MDCTXEmpty, EVP_MD_CTX_NNnode. Exists md; entailer. cancel.
+        rewrite if_false by trivial.
+        unfold EVP_MD_rep, EVP_MD_NNnode. Exists dsh dvals. entailer!. }
+Time Qed. (*22s*)
+
+Lemma subsume_EVP_DigestInit:
+      subsume_funspec (snd EVP_DigestInit_SPEC) (snd EVP_DigestInit_ASPEC).
+Proof.
+apply NDsubsume_subsume.
+{ split; reflexivity. }
+split3; auto.
+intros [[[gv ctx] t] T]. rewrite EVP_MD_rep_isptr'; Intros. rename H into SCT.
+  replace_SEP 0 (MDCTXAllocated ctx) by entailer!.
+  unfold MDCTXAllocated; Intros.
+  Exists (ctx, t, T, gv, Ews) (OPENSSL_malloc_token 16 ctx).
+  apply andp_right; auto.
+  - old_go_lower. entailer!.
+  - apply prop_right. Intros rv. Exists rv. simplify_Delta. 
+    old_go_lower. Intros; subst. apply andp_right. apply prop_right; intuition. cancel.
+    unfold DIE_postMpred; simpl.
+    rewrite sepcon_comm, distrib_orp_sepcon. apply orp_left.
+    * Intros; subst. rewrite if_true by trivial. unfold MDCTXRaw, CTX_NULL. cancel.
+    * Intros m; subst. rewrite if_false by discriminate.
+      rewrite OPENSSL_malloc_token_compatible' with (v:=m); Intros. 
+      apply andp_right. apply prop_right; trivial.
+      Exists m. cancel.  unfold EVP_MD_CTX_NNnode. entailer!.
+Qed. (*
+Lemma subsume_EVP_DigestInit:
+      subsume_funspec (snd EVP_DigestInit_SPEC) (snd EVP_DigestInit_ASPEC).
+Proof.
+apply NDsubsume_subsume.
+{ split; reflexivity. }
+split3; auto.
+intros [[[[gv ctx] t] T] c]. rewrite EVP_MD_rep_isptr'; Intros. rename H into SCT.
+destruct c.
++ (*Allocated*)
+  replace_SEP 0 (MDCTXAllocated ctx) by entailer!. 
+  unfold MDCTXAllocated; Intros.
+  Exists (ctx, t, T, gv, Ews) (OPENSSL_malloc_token 16 ctx).
+  apply andp_right; auto.
+  - old_go_lower. entailer!.
+  - apply prop_right. Intros rv. Exists rv. simplify_Delta. 
+    old_go_lower. Intros; subst. apply andp_right. apply prop_right; intuition. cancel.
+    unfold DIE_postMpred; simpl.
+    rewrite sepcon_comm, distrib_orp_sepcon. apply orp_left.
+    * Intros; subst. rewrite if_true by trivial. unfold MDCTXRaw, CTX_NULL. cancel.
+    * Intros m; subst. rewrite if_false by discriminate.
+      rewrite OPENSSL_malloc_token_compatible' with (v:=m); Intros. 
+      apply andp_right. apply prop_right; trivial.
+      Exists m. cancel.  unfold EVP_MD_CTX_NNnode. entailer!.
++ (*Raw*) 
+  replace_SEP 0 (MDCTXRaw ctx) by entailer!. 
+  unfold MDCTXRaw, CTX_NULL; Intros.
+  Exists (ctx, t, T, gv, Ews) (OPENSSL_malloc_token 16 ctx).
+  apply andp_right; auto.
+  - old_go_lower. entailer!.
+  - apply prop_right. Intros rv. Exists rv. simplify_Delta.
+    old_go_lower. entailer!.
+    unfold DIE_postMpred; simpl. 
+    rewrite sepcon_comm, distrib_orp_sepcon. apply orp_left.
+    * Intros; subst. rewrite if_true by trivial. unfold MDCTXRaw, CTX_NULL. cancel.
+    * Intros m; subst. rewrite if_false by discriminate. entailer!.
+      rewrite OPENSSL_malloc_token_compatible' with (v:=m); Intros.
+      Exists m. cancel. unfold EVP_MD_CTX_NNnode; entailer!.
++ (*Empty*) 
+  replace_SEP 0 (MDCTXEmpty D d ctx) by entailer!. 
+  unfold MDCTXEmpty; Intros md.
+  Exists (ctx, t, T, gv, Ews) (OPENSSL_malloc_token 16 ctx * MD_state Ews (INI D) md * OPENSSL_malloc_token (ctx_size_of_MD D) md).
+  apply andp_right; auto.
+  - old_go_lower. Intros. cancel. subst. apply andp_right. apply prop_right; intuition. cancel.
+  - apply prop_right. Intros rv. Exists rv. simplify_Delta.
+    old_go_lower. entailer!. 
+    Exists md. cancel. unfold DIE_postMpred; simpl.
+    rewrite sepcon_comm, distrib_orp_sepcon. apply orp_left.
+    * Intros; subst. rewrite if_true by trivial.
+      unfold MDCTXRaw, CTX_NULL. entailer!.
+    * Intros m; subst. rewrite if_false by discriminate. entailer!.
+      rewrite OPENSSL_malloc_token_compatible' with (v:=m); Intros.
+      Exists m. cancel. unfold EVP_MD_CTX_NNnode; entailer!.
++ (*Hashed*) 
+  replace_SEP 0 (MDCTXHashed DC d ctx) by entailer!. 
+  unfold MDCTXHashed; Intros md.
+  Exists (ctx, t, T, gv, Ews) (OPENSSL_malloc_token 16 ctx * MD_state Ews DC md * OPENSSL_malloc_token (ctx_size_of_MD (__EVP_MD DC)) md).
+  apply andp_right; auto.
+  - old_go_lower. Intros. apply andp_right. apply prop_right; intuition. cancel.
+  - apply prop_right. Intros rv. Exists rv. simplify_Delta. 
+    old_go_lower. simpl; Intros. apply andp_right. apply prop_right; intuition. 
+    cancel. unfold DIE_postMpred. simpl.
+    rewrite sepcon_comm, distrib_orp_sepcon. apply orp_left.
+    * Intros; subst. rewrite if_true by trivial.
+      Exists md; unfold MDCTXRaw, CTX_NULL. cancel.
+    * Exists md. cancel. subst _id. Intros m; subst. rewrite if_false by discriminate.
+      apply andp_right. apply prop_right; trivial.
+      rewrite OPENSSL_malloc_token_compatible' with (v:=m); Intros.
+      unfold MDCTXEmpty, EVP_MD_CTX_NNnode.
+      Exists m. cancel. entailer!.
++ (*Full*) 
+  replace_SEP 0 (MDCTXFull D d ctx) by entailer!. 
+  unfold MDCTXFull; Intros md.
+  unfold postFin; Intros findata.
+  Exists (ctx, t, T, gv, Ews) 
+         (OPENSSL_malloc_token 16 ctx * 
+          data_at Ews (__type findata) (__values findata) md * 
+          OPENSSL_malloc_token (ctx_size_of_MD D) md).
+  apply andp_right; auto.
+  - old_go_lower. Intros. apply andp_right. apply prop_right; intuition. cancel.
+  - apply prop_right. Intros rv. Exists rv. simplify_Delta.
+    old_go_lower; entailer; cancel. Exists md.
+    entailer!. Exists findata. cancel. unfold DIE_postMpred. simpl. 
+    rewrite sepcon_comm, distrib_orp_sepcon. apply orp_left.
+    * Intros; subst. rewrite if_true by trivial. cancel.
+      unfold MDCTXRaw, CTX_NULL. cancel. 
+    * Intros m; subst. rewrite if_false by discriminate.
+      rewrite OPENSSL_malloc_token_compatible' with (v:=m); Intros.
+      apply andp_right. apply prop_right; intuition.
+      Exists m. cancel. unfold EVP_MD_CTX_NNnode; entailer!.
+Qed.*)
+
+End EVP_MD_CTX_Protocol.
+(*
+(*TODO (discuss): we don't have a entailment converting configured (and hence hashed or finished) 
+contexts into initialized (and hence allocated) contexts, fnullval: r two reasons:
+a) it would leak the md memory region in the postcondition
+b) configured requires d, md to me pointer_or_null. Initialized requires them to be null.
+Thus, users are forced to use EVM_MD_CTX_cleanup to perform this conversion
+*)
+(*
+Definition MDCTXHashed D (data:list Z) (d p:val): mpred :=
+  EX md:val, EX v: reptype (struct_of_MD D),
+       !!(MD_proper D /\ DigestRep (struct_of_MD D) v data)
+       && EVP_MD_CTX_NNnode Tsh (d,(md,(nullval,nullval))) p *
+             data_at Tsh (struct_of_MD D) v md.*)
+(*Definition MDCTXHashed sh mdsh (DC: MD_with_content) (d p:val): mpred :=
+  EX md:val, (*!!(MD_proper D) &&*) 
+     !!(readable_share sh /\ writable_share mdsh) 
+     && EVP_MD_CTX_NNnode sh (d,(md,(nullval,nullval))) p *
+        OPENSSL_malloc_token 16 p *
+        MD_state mdsh DC md * OPENSSL_malloc_token (ctx_size_of_MD (__EVP_MD DC)) md.*)
+
+Variant ConfHashedFinished D:=
+  Configured: ConfHashedFinished D
+| Hashed: (mddataTp D) -> ConfHashedFinished D
+| Finished: (mddataTp D) -> ConfHashedFinished D.
+
+Variant EVP_DigestInit_ex_case:=
+  DIEx_CaseINI: EVP_DigestInit_ex_case (*ctx has been initialized but not been configured*)
+| DIEx_CaseSameMD: EVP_DigestInit_ex_case (*ctx presently configured to same MD we want to initialize to*)
+| DIEx_CaseDiffMD: forall (D:EVP_MD) (d:val) (p:ConfHashedFinished D), EVP_DigestInit_ex_case. (*ctx presently configured to MD D at d
+            and these are different from what we want*)
+
+Definition ConfHashedFinishedMpred D d p ctx :=
+           match p with
+           | Configured => MDCTXConfigured D d ctx
+           | Hashed data => MDCTXHashed (Build_MD_with_content D data) d ctx
+           | Finished data => MDCTXFinished (Build_MD_with_content D data) d ctx
+           end.
+
+Definition EVP_DigestInitExPre T t (c:EVP_DigestInit_ex_case) ctx :=
+  match c with 
+  DIEx_CaseINI => MDCTXInitialized ctx
+| DIEx_CaseSameMD => MDCTXConfigured T t ctx || EX data:_, MDCTXFinished (Build_MD_with_content T data) t ctx
+| DIEx_CaseDiffMD D d p => 
+       !!(d<>t /\ D<>T) && ConfHashedFinishedMpred D d p ctx * EVP_MD_rep D d  
+  end.
+
+Definition EVP_DigestInitExPost T t (c:EVP_DigestInit_ex_case) rv ctx :=
+  match c with 
+  DIEx_CaseINI => (!!(rv= nullval) && MDCTXInitialized ctx)
+               || (!!(rv= Vint Int.one) && MDCTXHashed (INI T) t ctx)
+| DIEx_CaseSameMD => !!(rv= Vint Int.one) && MDCTXHashed (INI T) t ctx
+| DIEx_CaseDiffMD D d p => 
+       (!!(rv= nullval) && ConfHashedFinishedMpred D d p ctx * EVP_MD_rep D d)
+    || (!!(rv= Vint Int.one) && MDCTXHashed (INI T) t ctx * EVP_MD_rep D d)
+  end.
+
+(*Header file specifies that ictx must already be initialized*)
+Definition EVP_DigestInit_ex_ASPEC := DECLARE _EVP_DigestInit_ex
+  WITH gv:globals, ctx:val, t:val, e:val, T: EVP_MD,
+       c: EVP_DigestInit_ex_case
+  PRE [ _ctx OF tptr (Tstruct _env_md_ctx_st noattr), 
+        _type OF tptr (Tstruct _env_md_st noattr),
+        _engine OF tptr (Tstruct _engine_st noattr) ]
+      PROP (4 <= ctx_size_of_MD T <= Int.max_unsigned - (WA + WORD) - 8)
+      LOCAL (gvars gv; temp _type t; temp _ctx ctx; temp _engine e)
+      SEP (EVP_DigestInitExPre T t c ctx; ERRGV gv; 
+           EVP_MD_rep T t; mm_inv gv)
+  POST [ tint] EX rv:_,
+       PROP ()
+       LOCAL (temp ret_temp rv)
+       SEP (EVP_DigestInitExPost T t c rv ctx; ERRGV gv; 
+            EVP_MD_rep T t; mm_inv gv).
+
+Lemma subsume_EVP_DigestInit_ex:
+      subsume_funspec (snd EVP_DigestInit_ex_SPEC) (snd EVP_DigestInit_ex_ASPEC).
+Proof. Admitted. (*
+apply NDsubsume_subsume.
+{ split; reflexivity. }
+split3; auto.
+intros [[[[[gv ctx] t] e] T] c]. rewrite EVP_MD_rep_isptr'; Intros. destruct c.
++ (*Case INI, ie initialized*)
+  replace_SEP 0 (MDCTXInitialized ctx). entailer!.
+  Intros; rename H into SC.
+  Exists (ctx, t, e, nullval, nullval, (nullval, nullval), T, gv, Ews, DIEC_NEQ None None)
+         (OPENSSL_malloc_token 16 ctx).
+  apply andp_right; auto.
+  - old_go_lower. entailer!.
+    unfold MDCTXInitialized, CTX_NULL; entailer!.
+  - apply prop_right. Intros rv. Exists rv. simplify_Delta. unfold DIE_postMpred.
+    old_go_lower; entailer; cancel.
+    rewrite sepcon_comm, distrib_orp_sepcon. apply orp_left.
+    * apply orp_right1. entailer!. unfold MDCTXInitialized, CTX_NULL; cancel.
+    * Intros m; apply orp_right2. rewrite OPENSSL_malloc_token_compatible'; Intros.
+      entailer!. unfold MDCTXHashed.
+      Exists m. cancel.
+      unfold EVP_MD_CTX_NNnode. entailer.
++ (*Case SameMD, ie configured/hashed or finished*)
+  replace_SEP 0 (EX md : val,
+ (EX data : mddataTp T,
+  EVP_MD_CTX_NNnode Ews (t, (md, (nullval, nullval))) ctx *
+  OPENSSL_malloc_token 16 ctx *
+  (*MD_state Ews {| __EVP_MD := T; __content := data |} md **) memory_block Ews (ctx_size_of_MD T) md *
+  OPENSSL_malloc_token (ctx_size_of_MD T) md)).
+   (*MDCTXConfigured T t ctx || EX data:_, MDCTXFinished (Build_MD_with_content T data) t ctx). entailer!.*)
+  { entailer!. simpl in *. apply orp_left.
+    + unfold MDCTXConfigured. Intros md data. Exists md data. unfold EVP_MD_CTX_NNnode. entailer!. admit.
+    + unfold MDCTXFinished. Intros data md. Exists md data. 
+      rewrite OPENSSL_malloc_token_compatible' with (v:=md); Intros. entailer!. simpl. cancel. admit. }
+
+  rename H into SZ. Intros m c.
+    rewrite OPENSSL_malloc_token_compatible' with (v:=m); Intros. 
+    Exists (ctx, t, e, t, m, (nullval, nullval), T, gv, Ews, DIEC_EQ)
+           (OPENSSL_malloc_token 16 ctx * mm_inv gv * OPENSSL_malloc_token (ctx_size_of_MD T) m).
+    apply andp_right; auto.
+    - old_go_lower. entailer. cancel. Search preInit. admit. (* entailer.
+      eapply derives_trans. apply MD_state_memoryblock. simpl. apply preInit_fresh_EWS.*)
+    - apply prop_right. Intros rv. Exists rv. simplify_Delta. unfold DIE_postMpred.
+      old_go_lower; entailer; cancel. 
+      Exists m. cancel.
+      unfold EVP_MD_CTX_NNnode. simpl. entailer!.
++ (*Case diffMD, ie configured or hashed*)
+  replace_SEP 0 (!!(d<>t /\ D<>T) && ConfHashedFinishedMpred D d p ctx * EVP_MD_rep D d). entailer!.
+  Intros. rename H into SZ. rename H0 into dt; rename H1 into DT.
+  destruct p as [ | data | data].
+  { (*Configured*)
+    replace_SEP 0 (MDCTXConfigured D d ctx). entailer!.
+    unfold MDCTXConfigured, EVP_MD_rep. Intros m c sh vals. rename H into Rsh.
+    Exists (ctx, t, e, d, m, (nullval, nullval), T, gv, Ews, DIEC_NEQ (Some (sh,vals)) (Some {| __EVP_MD := D; __content := c |}))
+           (OPENSSL_malloc_token 16 ctx * match_EVP_MD D vals).
+    apply andp_right; auto.
+    - old_go_lower. entailer!. unfold EVP_MD_NNnode. entailer!.
+    - apply prop_right. Intros rv. Exists rv. simplify_Delta. unfold DIE_postMpred. 
+      old_go_lower; entailer.
+      Exists x x0. entailer!.
+      rewrite sepcon_comm. do 2 rewrite <- sepcon_assoc. rewrite sepcon_comm. 
+      rewrite distrib_orp_sepcon. apply orp_left.
+      * Intros; apply orp_right1; unfold MDCTXConfigured, EVP_MD_rep, EVP_MD_NNnode, EVP_MD_CTX_NNnode; entailer!.
+        rewrite OPENSSL_malloc_token_compatible'; Intros.
+        Exists sh m c vals. entailer!.
+      * normalize. rewrite OPENSSL_malloc_token_compatible'; Intros. apply orp_right2. entailer!.
+        unfold MDCTXHashed, EVP_MD_rep, EVP_MD_NNnode, EVP_MD_CTX_NNnode; entailer!.
+        Exists sh x1 vals; simpl. entailer!. }
+  { (*Hashed*) 
+    replace_SEP 0 (MDCTXHashed {| __EVP_MD := D; __content := data |} d ctx). entailer!.
+    unfold MDCTXHashed. Intros m. unfold EVP_MD_rep at 1. 
+    Intros dsh dvals. rename H into Rdsh.
+    Exists (ctx, t, e, d, m, (nullval, nullval), T, gv, Ews, DIEC_NEQ (Some(dsh,dvals)) (Some {| __EVP_MD := D; __content := data |}))
+         (OPENSSL_malloc_token 16 ctx * match_EVP_MD D dvals).
+    apply andp_right; auto.
+    - old_go_lower. entailer!. unfold EVP_MD_NNnode. entailer!.
+    - apply prop_right. Intros rv. Exists rv. simplify_Delta. old_go_lower; entailer. cancel.
+      unfold DIE_postMpred. simpl.
+      rewrite sepcon_comm. do 3 rewrite <- sepcon_assoc. rewrite sepcon_comm.
+      rewrite distrib_orp_sepcon. apply orp_left.
+      * Intros; apply orp_right1. unfold MDCTXHashed, EVP_MD_NNnode.
+        rewrite OPENSSL_malloc_token_compatible'; Intros. Exists m; entailer. simpl; cancel.
+        entailer!.
+        unfold EVP_MD_rep. Exists dsh dvals. entailer!.
+      * normalize. rewrite OPENSSL_malloc_token_compatible'; Intros. apply orp_right2. entailer!.
+        unfold MDCTXHashed, EVP_MD_rep, EVP_MD_NNnode, EVP_MD_CTX_NNnode; entailer!.
+        Exists dsh x dvals; simpl. entailer!. }
+  { (*Finished*) 
+    replace_SEP 0 (MDCTXFinished {| __EVP_MD := D; __content := data |} d ctx). entailer!.
+    unfold MDCTXFinished. Intros m. unfold EVP_MD_rep at 1. 
+    Intros dsh dvals. rename H into Rdsh.
+    Exists (ctx, t, e, d, m, (nullval, nullval), T, gv, Ews, DIEC_NEQ (Some(dsh,dvals)) (Some {| __EVP_MD := D; __content := data |}))
+         (OPENSSL_malloc_token 16 ctx * match_EVP_MD D dvals).
+    apply andp_right; auto.
+    - old_go_lower. entailer!. unfold EVP_MD_NNnode. entailer!.
+    - apply prop_right. Intros rv. Exists rv. simplify_Delta. old_go_lower; entailer. cancel.
+      unfold DIE_postMpred. simpl.
+      rewrite sepcon_comm. do 3 rewrite <- sepcon_assoc. rewrite sepcon_comm.
+      rewrite distrib_orp_sepcon. apply orp_left.
+      * Intros; apply orp_right1. unfold MDCTXHashed, EVP_MD_NNnode.
+        rewrite OPENSSL_malloc_token_compatible'; Intros. Exists m; entailer. simpl; cancel.
+        entailer!.
+        unfold EVP_MD_rep. Exists dsh dvals. entailer!.
+      * normalize. rewrite OPENSSL_malloc_token_compatible'; Intros. apply orp_right2. entailer!.
+        unfold MDCTXHashed, EVP_MD_rep, EVP_MD_NNnode, EVP_MD_CTX_NNnode; entailer!.
+        Exists dsh x dvals; simpl. entailer!. }
+Time Qed. (*3.1s*)*)
+(*
+Variant EVP_DigestInit_case:=
+  DI_CaseAlloc: EVP_DigestInit_case (*ctx has been allocated or initialized but not configured*)
+| DI_CaseConf: forall D (d:val) (p:ConfOrHashed D), EVP_DigestInit_case. (*ctx has been configured*)
+
+Definition EVP_DigestInitPre (c:EVP_DigestInit_case) ctx :=
+  match c with 
+  DI_CaseAlloc => MDCTXAllocated ctx
+| DI_CaseConf D d p => ConfOrHashedMpred D d p ctx
+  end.
+
+Definition EVP_DigestInitPost T t (c:EVP_DigestInit_case) rv ctx :=
+  match c with 
+  DI_CaseAlloc => (!!(rv= nullval) && MDCTXInitialized ctx)
+               || (!!(rv= Vint Int.one) && MDCTXHashed (INI T) t ctx)
+| DI_CaseConf D d p => 
+           (    (!!(rv= nullval) && MDCTXInitialized ctx)
+             || (!!(rv= Vint Int.one) && MDCTXHashed (INI T) t ctx) )
+           * EX md:_, EX data:_, 
+             !!(match p with Configured => True | Hashed data' =>  data=data' end) &&
+             MD_state Ews {| __EVP_MD := D; __content := data |} md * 
+             OPENSSL_malloc_token (ctx_size_of_MD D) md  (*IS THIS A MEMORY LEAK?*)
+  end.
+
+Definition EVP_DigestInit_ASPEC := DECLARE _EVP_DigestInit
+  WITH gv:globals, ctx:val, t:val, T: EVP_MD, c: EVP_DigestInit_case
+  PRE [ _ctx OF tptr (Tstruct _env_md_ctx_st noattr), 
+        _type OF tptr (Tstruct _env_md_st noattr) ]
+      PROP (4 <= ctx_size_of_MD T <= Int.max_unsigned - (WA + WORD) - 8)
+      LOCAL (gvars gv; temp _type t; temp _ctx ctx)
+      SEP (EVP_DigestInitPre c ctx; ERRGV gv; EVP_MD_rep T t; mm_inv gv)
+  POST [ tint] EX rv:_,
+       PROP ()
+       LOCAL (temp ret_temp rv)
+       SEP (EVP_DigestInitPost T t c rv ctx; ERRGV gv; EVP_MD_rep T t; mm_inv gv).
+
+Lemma subsume_EVP_DigestInit:
+      subsume_funspec (snd EVP_DigestInit_SPEC) (snd EVP_DigestInit_ASPEC).
+Proof.
+apply NDsubsume_subsume.
+{ split; reflexivity. }
+split3; auto.
+intros [[[[gv ctx] t] T] c]. rewrite EVP_MD_rep_isptr'; Intros. rename H into SZ.
+destruct c.
++ (*Alloc*)
+  replace_SEP 0 (MDCTXAllocated ctx). entailer!.
+  unfold MDCTXAllocated.
+  Exists (ctx, t, T, gv, Ews) (OPENSSL_malloc_token 16 ctx).
+  apply andp_right.
+  * old_go_lower; entailer!.
+  * apply prop_right. simplify_Delta. Intros rv; Exists rv. old_go_lower; entailer!.
+    unfold DIE_postMpred; simpl.
+    rewrite sepcon_comm, distrib_orp_sepcon; apply orp_left.
+    - Intros; apply orp_right1. unfold MDCTXInitialized, CTX_NULL; entailer!.
+    - Intros m; apply orp_right2. rewrite OPENSSL_malloc_token_compatible'; Intros.
+      unfold MDCTXHashed. Exists m; simpl; entailer!.
++ (*Conf*) 
+  replace_SEP 0 (ConfOrHashedMpred D d p ctx). entailer!.
+  destruct p as [ | data].
+  { (*Configured*)
+    replace_SEP 0 (MDCTXConfigured D d ctx). entailer!. 
+    unfold MDCTXConfigured, EVP_MD_CTX_NNnode; Intros md data.
+    sep_apply (data_at_data_at_ Ews (Tstruct _env_md_ctx_st noattr) (d, (md, (nullval, nullval))) ctx).
+    Exists (ctx, t, T, gv, Ews)
+           (OPENSSL_malloc_token 16 ctx * MD_state Ews {| __EVP_MD := D; __content := data |} md * OPENSSL_malloc_token (ctx_size_of_MD D) md).
+    apply andp_right.
+    * old_go_lower; entailer!.
+    * apply prop_right. simplify_Delta. Intros rv; Exists rv. old_go_lower; entailer. Exists md data. entailer!.
+      unfold DIE_postMpred; simpl.
+      rewrite sepcon_comm, distrib_orp_sepcon; apply orp_left.
+      - Intros; subst. apply orp_right1. unfold MDCTXInitialized, CTX_NULL; entailer!.
+      - Intros m; apply orp_right2. rewrite OPENSSL_malloc_token_compatible'; Intros; entailer!.
+        unfold MDCTXHashed. Exists m; simpl; entailer!. }
+  { (*Hashed*)
+    replace_SEP 0 (MDCTXHashed {| __EVP_MD := D; __content := data |} d ctx). entailer!. 
+    unfold MDCTXHashed, EVP_MD_CTX_NNnode; Intros md.
+    sep_apply (data_at_data_at_ Ews (Tstruct _env_md_ctx_st noattr) (d, (md, (nullval, nullval))) ctx).
+    Exists (ctx, t, T, gv, Ews)
+           (OPENSSL_malloc_token 16 ctx * MD_state Ews {| __EVP_MD := D; __content := data |} md * OPENSSL_malloc_token (ctx_size_of_MD D) md).
+    apply andp_right.
+    * old_go_lower; entailer!.
+    * apply prop_right. simplify_Delta. Intros rv; Exists rv. old_go_lower; entailer. Exists md data. entailer!.
+      unfold DIE_postMpred; simpl.
+      rewrite sepcon_comm, distrib_orp_sepcon; apply orp_left.
+      - Intros; subst. apply orp_right1. unfold MDCTXInitialized, CTX_NULL; entailer!.
+      - Intros m; apply orp_right2. rewrite OPENSSL_malloc_token_compatible'; Intros; entailer!.
+        unfold MDCTXHashed. Exists m; simpl; entailer!. }
+Qed.
+*)
+Definition EVP_DigestUpdate_ASPEC := DECLARE _EVP_DigestUpdate
+  WITH ctx: val, t:val, d: val, dsh:share, data: list byte, DC: MD_with_content, len:Z
+  PRE [ _ctx OF tptr (Tstruct _env_md_ctx_st noattr), _data OF tptr tvoid,  _len OF tuint ]
+      PROP (readable_share dsh; UpdateSideconditions DC data len)
+      LOCAL (temp _ctx ctx; temp _data d; temp _len (Vint (Int.repr len)) )
+      SEP (MDCTXHashed DC t ctx; data_block dsh data d; EVP_MD_rep (__EVP_MD DC) t)
+  POST [ tint] 
+       PROP ()
+       LOCAL (temp ret_temp (Vint Int.one))
+       SEP (MDCTXHashed (UPD DC data len) t ctx; data_block dsh data d; EVP_MD_rep (__EVP_MD DC) t).
+
+Lemma subsume_EVP_DigestUpdate:
+      subsume_funspec (snd EVP_DigestUpdate_SPEC) (snd EVP_DigestUpdate_ASPEC).
+Proof.
+apply NDsubsume_subsume.
+{ split; reflexivity. }
+split3; auto.
+intros [[[[[[ctx t] d] dsh] data] DC] len]. 
+rewrite EVP_MD_rep_isptr'; Intros. rename H into Rdsh. rename H0 into SC.
+unfold MDCTXHashed, EVP_MD_CTX_NNnode; Intros md.
+Exists (ctx, Ews, (t, (md, (nullval, nullval))), d, dsh, data, DC, len, Ews)
+       (OPENSSL_malloc_token (ctx_size_of_MD (__EVP_MD DC)) md * OPENSSL_malloc_token 16 ctx).
+apply andp_right.
++ old_go_lower; entailer!.
++ apply prop_right. simplify_Delta. old_go_lower; entailer. Exists md. entailer!.
+Qed.
+
+Definition EVP_DigestFinal_ex_ASPEC := DECLARE _EVP_DigestFinal_ex
+  WITH ctx: val, t:val, 
+       out: val, osh:share, sz:val,
+       DC:MD_with_content
+  PRE [ _ctx OF tptr (Tstruct _env_md_ctx_st noattr),
+        _md_out OF tptr tuchar, _size OF tptr tuint]
+      PROP (writable_share osh;
+            0 <= ctx_size_of_MD (__EVP_MD DC) <= Int.max_unsigned)
+      LOCAL (temp _ctx ctx; temp _md_out out; temp _size sz )
+      SEP (MDCTXHashed DC t ctx; EVP_MD_rep (__EVP_MD DC) t;
+           if Val.eq sz nullval then emp else data_at_ Ews tuint sz;
+           memory_block osh (md_size_of_MD (__EVP_MD DC)) out)
+  POST [ tint] 
+       PROP ()
+       LOCAL (temp ret_temp (Vint Int.one))
+       SEP (MDCTXFinished DC t ctx;
+            EVP_MD_rep (__EVP_MD DC) t;
+            if Val.eq sz nullval then emp else data_at Ews tuint (Vint (Int.repr (md_size_of_MD (__EVP_MD DC)))) sz;
+            data_block osh (FIN DC) out).
+
+Lemma subsume_EVP_DigestFinal_ex:
+      subsume_funspec (snd EVP_DigestFinal_ex_SPEC) (snd EVP_DigestFinal_ex_ASPEC).
+Proof.
+apply NDsubsume_subsume.
+{ split; reflexivity. }
+split3; auto.
+intros [[[[[ctx t] out] osh] sz] DC].
+rewrite EVP_MD_rep_isptr'; Intros. rename H into Wosh. rename H0 into SZ.
+unfold MDCTXHashed, EVP_MD_CTX_NNnode; Intros md.
+Exists (ctx, Ews, (t, (md, (nullval, nullval))), out, osh, sz, DC, Ews)
+       (OPENSSL_malloc_token (ctx_size_of_MD (__EVP_MD DC)) md * OPENSSL_malloc_token 16 ctx).
+apply andp_right.
++ old_go_lower; entailer!.
++ apply prop_right. simplify_Delta. old_go_lower; entailer!. Exists md; cancel.
+Qed.
+
+Definition EVP_DigestFinal_ASPEC := DECLARE _EVP_DigestFinal
+  WITH gv: globals, ctx: val, t:val, 
+       out: val, osh:share, sz:val,
+       DC:MD_with_content
+  PRE [_ctx OF tptr (Tstruct _env_md_ctx_st noattr),
+        _md OF tptr tuchar, _size OF tptr tuint]
+      PROP (writable_share osh;
+            0 <= ctx_size_of_MD (__EVP_MD DC) <= Int.max_unsigned)
+      LOCAL (gvars gv; temp _ctx ctx; temp _md out; temp _size sz )
+      SEP (MDCTXHashed DC t ctx; EVP_MD_rep (__EVP_MD DC) t;
+           if Val.eq sz nullval then emp else data_at_ Ews tuint sz;
+           memory_block osh (md_size_of_MD (__EVP_MD DC)) out; mm_inv gv)
+  POST [ tint] 
+       PROP ()
+       LOCAL (temp ret_temp (Vint Int.one))
+       SEP (MDCTXInitialized ctx;
+            EVP_MD_rep (__EVP_MD DC) t;
+            if Val.eq sz nullval then emp else data_at Ews tuint (Vint (Int.repr (md_size_of_MD (__EVP_MD DC)))) sz;
+            data_block osh (FIN DC) out; mm_inv gv).
+
+Lemma subsume_EVP_DigestFinal:
+      subsume_funspec (snd EVP_DigestFinal_SPEC) (snd EVP_DigestFinal_ASPEC).
+Proof.
+apply NDsubsume_subsume.
+{ split; reflexivity. }
+split3; auto.
+intros [[[[[[gv ctx] t] out] osh] sz] DC].
+rewrite EVP_MD_rep_isptr'; Intros. rename H into Wosh. rename H0 into SZ.
+unfold MDCTXHashed, EVP_MD_CTX_NNnode; Intros md.
+Exists (gv, ctx, Ews, (t, (md, (nullval, nullval))), out, osh, sz, DC)
+       (OPENSSL_malloc_token 16 ctx).
+apply andp_right.
++ old_go_lower; entailer!.
++ apply prop_right. simplify_Delta. old_go_lower; entailer!.
+  unfold MDCTXInitialized; cancel.
+Qed.
+
+(*free can't be called on a merely allocated (but not yet initialized) CTX -- the md field is Vundef*)
+Inductive EVP_MD_CTX_free_case :=
+(*  FreeNull: EVP_MD_CTX_free_case TODO: should this be supported? If we're supporting it here, what about the other operations?*)
+  FreeInitialized: EVP_MD_CTX_free_case
+| FreeConfiguredOrFinished: forall (D:EVP_MD) (d:val), EVP_MD_CTX_free_case.
+
+Definition EVP_MD_CTX_free_pre (c:EVP_MD_CTX_free_case) (ctx:val) : mpred :=
+  match c with
+(* | FreeNull: !!(ctx=nullval) && emp)*)
+ | FreeInitialized => MDCTXInitialized ctx
+ | FreeConfiguredOrFinished D d => 
+      MDCTXConfigured D d ctx (*|| MDCTXFinished D d ctx*)
+  end.
+
+Definition EVP_MD_CTX_free_ASPEC := DECLARE _EVP_MD_CTX_free
+  WITH gv:globals, ctx:val, c: EVP_MD_CTX_free_case
+  PRE [ _ctx OF (tptr (Tstruct _env_md_ctx_st noattr)) ]
+      PROP ()
+      LOCAL (gvars gv; temp _ctx ctx)
+      SEP (EVP_MD_CTX_free_pre c ctx; mm_inv gv)
+  POST [ tvoid ]
+       PROP ()
+       LOCAL ()
+       SEP (mm_inv gv).
+
+Inductive EVP_MD_CTX_cleanup_case :=
+  ClInitialized: EVP_MD_CTX_cleanup_case
+| ClConfiguredOrFinished: forall (D:EVP_MD) (d:val), EVP_MD_CTX_cleanup_case.
+
+Definition EVP_MD_CTX_cleanup_pre (c:EVP_MD_CTX_cleanup_case) (ctx:val) : mpred :=
+  match c with
+   ClInitialized => MDCTXInitialized ctx (*Note: can't use ALLOCATED here: the body's first instruction accesses ctx -> md_data*)
+ | ClConfiguredOrFinished D d => 
+      (MDCTXConfigured D d ctx (*|| MDCTXFinished D d ctx*)) * EVP_MD_rep D d
+end.
+
+Definition EVP_MD_CTX_cleanup_post (c:EVP_MD_CTX_cleanup_case) (ctx:val) : mpred :=
+  match c with
+   ClInitialized => MDCTXInitialized ctx
+ | ClConfiguredOrFinished D d => MDCTXInitialized ctx * EVP_MD_rep D d
+end.
+
+Definition EVP_MD_CTX_cleanup_ASPEC := DECLARE _EVP_MD_CTX_cleanup
+  WITH gv:globals, ctx:val, c:EVP_MD_CTX_cleanup_case
+  PRE [ _ctx OF (tptr (Tstruct _env_md_ctx_st noattr)) ]
+      PROP () LOCAL (gvars gv; temp _ctx ctx)
+      SEP (EVP_MD_CTX_cleanup_pre c ctx; mm_inv gv)
+  POST [ tint ]
+       PROP () LOCAL (temp ret_temp (Vint (Int.one)))
+       SEP (EVP_MD_CTX_cleanup_post c ctx; mm_inv gv).
+
+Definition EVP_MD_CTX_init_ASPEC := DECLARE _EVP_MD_CTX_init
+   WITH ctx:val
+   PRE [ _ctx OF tptr (Tstruct _env_md_ctx_st noattr) ]
+       PROP () LOCAL (temp _ctx ctx) SEP (MDCTXAllocated ctx)
+   POST [ tvoid ]
+       PROP () LOCAL () SEP (MDCTXInitialized ctx).
+
+(*Note that this is the same spec as cleanup! Indeed the comment in the header file
+  suggests that the precondition should be that of lceanup, whereas the fact that
+  cleanup results in an initialized (not merely allocated) ctx means that doing init again does not change much*)
+Definition EVP_MD_CTX_reset_ASPEC := DECLARE _EVP_MD_CTX_reset
+  WITH gv:globals, ctx:val, c: EVP_MD_CTX_cleanup_case
+  PRE [ _ctx OF (tptr (Tstruct _env_md_ctx_st noattr)) ]
+      PROP ()
+      LOCAL (gvars gv; temp _ctx ctx)
+      SEP (EVP_MD_CTX_cleanup_pre c ctx; mm_inv gv)
+  POST [ tint]
+       PROP ()
+       LOCAL (temp ret_temp (Vint Int.one))
+       SEP (EVP_MD_CTX_cleanup_post c ctx; mm_inv gv).
+
+Lemma subsume_EVP_MD_CTX_cleanup:
+      subsume_funspec (snd EVP_MD_CTX_cleanup_SPEC) (snd EVP_MD_CTX_cleanup_ASPEC).
+Proof.
+apply NDsubsume_subsume.
+{ split; reflexivity. }
+split3; auto.
+intros [[gv ctx] c]. destruct c.
++ (*Case ClInitialized*)
+  Exists (gv, ctx, Ews, nullval, @None Z) (OPENSSL_malloc_token 16 ctx).
+  apply andp_right; auto.
+  - old_go_lower. unfold MDCTXInitialized, CTX_NULL. entailer!.
+    Exists nullval nullval. entailer!. 
+  - entailer!. unfold MDCTXInitialized, CTX_NULL. entailer!.
++ (*Case ClConfiguredOrFinished*)
+  replace_SEP 0 (MDCTXConfigured D d ctx * EVP_MD_rep D d). 
+  { entailer!. } 
+  unfold MDCTXConfigured. Intros md data.
+  Exists (gv, ctx, Ews, md, Some (ctx_size_of_MD D)) (EVP_MD_rep D d * OPENSSL_malloc_token 16 ctx).
+  apply andp_right; auto.
+  - old_go_lower. Exists d nullval. entailer!. apply MD_state_memoryblock.
+  - apply prop_right. simplify_Delta. old_go_lower. entailer.
+    unfold MDCTXInitialized. cancel.
+Qed.
+
+(*Indeed - same proof as for cleanup*)
+Lemma subsume_EVP_MD_CTX_reset:
+      subsume_funspec (snd EVP_MD_CTX_reset_SPEC) (snd EVP_MD_CTX_reset_ASPEC).
+Proof.
+apply NDsubsume_subsume.
+{ split; reflexivity. }
+split3; auto.
+intros [[gv ctx] c]. destruct c.
++ (*Case ClInitialized*)
+  Exists (gv, ctx, Ews, nullval, @None Z) (OPENSSL_malloc_token 16 ctx).
+  apply andp_right; auto.
+  - old_go_lower. unfold MDCTXInitialized, CTX_NULL.
+    Exists nullval nullval. entailer!.
+  - entailer!. unfold MDCTXInitialized, CTX_NULL. entailer!.
++ (*Case ClConfiguredOrFinished*)
+  replace_SEP 0 (MDCTXConfigured D d ctx * EVP_MD_rep D d). 
+  { entailer!. } 
+  unfold MDCTXConfigured. Intros md data.
+  Exists (gv, ctx, Ews, md, Some (ctx_size_of_MD D)) (EVP_MD_rep D d * OPENSSL_malloc_token 16 ctx).
+  apply andp_right; auto.
+  - old_go_lower. Exists d nullval. entailer!. apply MD_state_memoryblock.
+  - apply prop_right. simplify_Delta. old_go_lower. entailer.
+    unfold MDCTXInitialized. cancel.
+Qed.
+
+Definition EVP_MD_CTX_newcreate_ASPEC :=
+   WITH gv:globals
+   PRE [ ]
+       PROP (24 <= Int.max_unsigned - (WA + WORD))
+       LOCAL (gvars gv)
+       SEP (mm_inv gv)
+   POST [ tptr (Tstruct _env_md_ctx_st noattr) ]
+     EX ctx:val,
+       PROP ()
+       LOCAL (temp ret_temp ctx)
+       SEP ((!!(ctx=nullval) && emp) || MDCTXInitialized ctx; mm_inv gv).
+
+Definition EVP_MD_CTX_create_ASPEC := DECLARE _EVP_MD_CTX_create EVP_MD_CTX_newcreate_ASPEC.
+Definition EVP_MD_CTX_new_ASPEC := DECLARE _EVP_MD_CTX_new EVP_MD_CTX_newcreate_ASPEC.
+
+Lemma subsume_EVP_MD_CTX_init:
+      subsume_funspec (snd EVP_MD_CTX_init_SPEC) (snd EVP_MD_CTX_init_ASPEC).
+Proof.
+apply NDsubsume_subsume.
+{ split; reflexivity. }
+split3; auto.
+intros ctx. Exists (ctx, Ews) (OPENSSL_malloc_token 16 ctx).
+apply andp_right; auto.
++ old_go_lower; entailer.
++ apply prop_right. simplify_Delta; old_go_lower. entailer.
+Qed.
+
+Lemma subsume_EVP_MD_CTX_create:
+      subsume_funspec (snd EVP_MD_CTX_create_SPEC) (snd EVP_MD_CTX_create_ASPEC).
+Proof.
+apply NDsubsume_subsume.
+{ split; reflexivity. }
+split3; auto.
+intros gv. Exists gv emp.
+change (`emp) with (@emp (environ->mpred) _ _); rewrite !emp_sepcon.
+apply andp_right; auto.
++ entailer!. 
++ apply prop_right. simplify_Delta. Intros ctx. Exists ctx. entailer.
+Qed.
+
+Lemma subsume_EVP_MD_CTX_new:
+      subsume_funspec (snd EVP_MD_CTX_new_SPEC) (snd EVP_MD_CTX_new_ASPEC).
+Proof.
+apply NDsubsume_subsume.
+{ split; reflexivity. }
+split3; auto.
+intros gv. Exists gv emp.
+change (`emp) with (@emp (environ->mpred) _ _); rewrite !emp_sepcon.
+apply andp_right; auto.
++ entailer!. 
++ apply prop_right. simplify_Delta. Intros ctx. Exists ctx. entailer.
+Qed.
+
+Lemma MDCTXAllocated_valid_ptr p: MDCTXAllocated p |-- valid_pointer p.
+Proof. unfold MDCTXAllocated. apply sepcon_valid_pointer2.
+  sep_apply (data_at__memory_block Ews (Tstruct _env_md_ctx_st noattr) p). Intros. simpl.
+  sep_apply (memory_block_valid_ptr Ews 16 p).
+  intuition. omega. trivial.
+Qed.
+
+Lemma MDCTXInitialized_valid_ptr p: MDCTXInitialized p |-- valid_pointer p.
+Proof. eapply derives_trans. apply InitializedAllocated. apply MDCTXAllocated_valid_ptr. Qed.
+
+Lemma MDCTXAllocated_isptr p: MDCTXAllocated p |-- !! isptr p.
+Proof. intros. unfold MDCTXAllocated. entailer!. Qed.
+
+Lemma MDCTXInitialized_isptr p: MDCTXInitialized p |-- !! isptr p.
+Proof. eapply derives_trans. apply InitializedAllocated. apply MDCTXAllocated_isptr. Qed.
+
+Lemma MDCTXAllocated_isptr' p: MDCTXAllocated p = (!!isptr p) && MDCTXAllocated p.
+Proof. apply pred_ext; entailer. apply MDCTXAllocated_isptr. Qed.
+
+Lemma MDCTXInitialized_isptr' p: MDCTXInitialized p = (!! isptr p) && MDCTXInitialized p.
+Proof. apply pred_ext; entailer. apply MDCTXInitialized_isptr. Qed.
+
+Lemma MDCTXConfigured_valid_ptr D d p: MDCTXConfigured D d p |-- valid_pointer p.
+Proof. unfold MDCTXConfigured, EVP_MD_CTX_NNnode. Intros md data.
+  apply sepcon_valid_pointer1; entailer!.
+Qed.
+
+Lemma MDCTXConfigured_isptr D d p: MDCTXConfigured D d p |-- !! isptr p.
+Proof. unfold MDCTXConfigured, EVP_MD_CTX_NNnode. Intros md data. entailer!. Qed.
+
+Lemma MDCTXFinished_valid_ptr D d p: MDCTXFinished D d p |-- valid_pointer p.
+Proof. unfold MDCTXFinished, EVP_MD_CTX_NNnode. Intros md.
+  apply sepcon_valid_pointer1. apply sepcon_valid_pointer2. entailer!. Qed.
+
+Lemma MDCTXFinished_isptr D d p: MDCTXFinished D d p |-- !! isptr p.
+Proof. unfold MDCTXFinished, EVP_MD_CTX_NNnode. Intros md. entailer!. Qed.
+
+End EVP_MD_CTX_Protocol.*)
