Makefile
@@ -370,7 +370,7 @@ FIPSDIGEST_FILES = \
   vstlib.v mem.v thread_none.v digest.v digests.v \
   digest_model.v spec_digest_base.v spec_mem.v verif_mem.v \
   spec_digest.v verif_digest.v verif_digests.v \
-  digest_protocol_spec.v
+  digest_protocol_spec.v digest_protocol_verif.v
 
 DIGEST_FILES = \
   digest.v digests.v digest_model.v spec_digests.v 
